EffectSSA/ProofSketch/LocalStack.lean
@@ -1,0 +1,121 @@
+module
+
+public import EffectSSA.ProofSketch.VarSet
+
+import Std.Data.HashMap
+
+/-!
+# LocalStack Structure
+
+This file defines a `LocalStack` structure, which is used to assign values to
+local (i.e, SSA) variables.
+-/
+namespace EffectSSA.ProofSketch
+public section
+
+open Std (HashMap)
+
+/-- `Val` is the type of runtime values -/
+axiom Val : Type
+
+def LocalStack.Raw :=
+  @Quot (Std.HashMap VarId Val) Std.HashMap.Equiv
+
+
+/-!
+## LocalStack Structure
+--------------------------------------------------------------------------------
+-/
+
+open LocalStack (Raw) in
+structure LocalStack where
+  raw : Raw
+
+namespace LocalStack
+
+def empty : LocalStack where
+  raw := Quot.mk _ (.mk {})
+instance : EmptyCollection LocalStack where emptyCollection := empty
+
+def contains (s : LocalStack) (v : VarId) : Bool :=
+  Quot.lift (·.contains v) (fun _ _ h => h.contains_eq) s.raw
+
+instance : Membership VarId LocalStack where
+  mem s v := s.contains v
+instance (v : VarId) (s : LocalStack) : Decidable (v ∈ s) :=
+  inferInstanceAs <| Decidable (s.contains v)
+
+@[simp, grind =]
+theorem mem_iff (s : LocalStack) (v : VarId) : v ∈ s ↔ s.contains v := by rfl
+
+def get? (s : LocalStack) (v : VarId) : Option Val :=
+  (Quot.lift (fun m : HashMap VarId Val => m[v]?) · s.raw) <| by
+    intro a b hab; exact hab.getElem?_eq
+
+def get (s : LocalStack) (v : VarId) (h : v ∈ s) : Val :=
+  (s.get? v).get <| by
+    obtain ⟨raw⟩ := s
+    cases raw using Quot.ind
+    case mk m =>
+      exact HashMap.mem_iff_isSome_getElem?.mp h
+
+instance : GetElem?  LocalStack VarId Val (fun s v => v ∈ s) where
+  getElem := get
+  getElem? := get?
+
+def insert (s : LocalStack) (v : VarId) (x : Val) : LocalStack where
+  raw := Quot.lift (fun m => Quot.mk _ (m.insert v x))
+    (fun _ _ h => Quot.sound (h.insert v x)) s.raw
+
+section Lemmas
+
+@[ext, grind ext]
+theorem ext {s t : LocalStack} : (h : ∀ v : VarId, s[v]? = t[v]?) → s = t := by
+  rcases s with ⟨s⟩
+  cases s using Quot.ind
+  case mk s =>
+  rcases t with ⟨t⟩
+  cases t using Quot.ind
+  case mk t =>
+  intro (h : ∀ v : VarId, s[v]? = t[v]?)
+  suffices s.Equiv t by
+    simp only [Quot.sound this]
+  apply HashMap.Equiv.of_forall_getElem?_eq h
+
+end Lemmas
+end LocalStack
+
+/-!
+## LocalStackT Monad Transformer
+--------------------------------------------------------------------------------
+-/
+@[expose] public section Expose
+
+abbrev LocalStackT := StateT LocalStack
+
+namespace LocalStackT
+variable {m} [Monad m]
+
+/--
+Read the value of variable `v` from the monadic state,
+returning `none` if `v` has no value assigned.
+-/
+def read? (v : VarId) : LocalStackT m (Option Val) := do
+  let ρ ← get
+  return ρ[v]?
+
+/--
+Assign value `x` to variable `v` in the monadic state.
+
+This is infallible, overwriting any value already present.
+-/
+def push (var : VarId) (val : Val) : LocalStackT m Unit :=
+  modify (·.insert var val)
+  -- NOTE: it seems tempting to throw an error here if `x` is already defined.
+  -- However, since we never remove variables, a variable being defined twice
+  -- does not necessarily indicate a mall-formed program. In particular, the
+  -- pre-existing value might actually come from the same instruction in
+  -- a previous iteration of a loop.
+
+end LocalStackT
+end Expose
